

Chapter 03 : Stirling Numbers

Section 1 : Stirling numbers of the second kind

Lemma 0.1 : Recursive relation

The stirling numbers of second kind satisfy the following recurrence

$$\left\{ \begin{matrix} n \\ k \end{matrix} \right\} = \left\{ \begin{matrix} n-1 \\ k-1 \end{matrix} \right\} + k \left\{ \begin{matrix} n-1 \\ k \end{matrix} \right\} \quad (1)$$

Proof is left as an exercise

Theorem 0.1 :

Let x be a variable :

$$x^n = \sum_{i=1}^n \left\{ \begin{matrix} n \\ i \end{matrix} \right\} (x)_i \quad (2)$$

Proof is left as an exercise

Section 2 : Stirling numbers of the third kind

Definition 1.1 :

The Stirling Numbers of the third kind (Lah numbers) , The Lah numbers count the number of ways to partition a set of n elements into k non empty lists (ordered subsets) , they are denoted $L(n, k)$ or $\left[\begin{matrix} n \\ k \end{matrix} \right]$

Lemma 1.1 :

Recurrence relation of Lah Numbers

$$\left[\begin{matrix} n \\ k \end{matrix} \right] = \left[\begin{matrix} n-1 \\ k-1 \end{matrix} \right] + (n+k-1) \left[\begin{matrix} n-1 \\ k \end{matrix} \right] \quad (1.1)$$

Theorem 1.1 :

Let x be a variable :

$$x^{(n)} = \sum_{k=1}^n \left[\begin{matrix} n \\ k \end{matrix} \right] (x)_k \quad (1.2)$$

Examples:

$$x(x+1) = x(x-1) + 2x \quad (1.3)$$

$$x(x+1)(x+2) = x(x-1)(x-2) + 6x(x-1) + 6x \quad (1.4)$$

Lemma 1.2 :

$$\left[\begin{matrix} n \\ k \end{matrix} \right] = \sum_{j=k}^n \left[\begin{matrix} n \\ j \end{matrix} \right] \left\{ \begin{matrix} j \\ k \end{matrix} \right\} \quad (1.5)$$

$$\begin{aligned} x^{(n)} &= \sum_{j=0}^n \left[\begin{matrix} n \\ j \end{matrix} \right] x^j \\ &= \sum_{j=0}^n \left[\begin{matrix} n \\ j \end{matrix} \right] \sum_{k=0}^j \left\{ \begin{matrix} j \\ k \end{matrix} \right\} (x)_k \\ x^{(n)} &= \sum_{k=0}^n \left[\sum_{j=k}^n \left[\begin{matrix} n \\ j \end{matrix} \right] \left\{ \begin{matrix} j \\ k \end{matrix} \right\} \right] (x)_k \end{aligned}$$

Some Notations:

$$\left[\begin{matrix} n \\ k \end{matrix} \right] = |\Delta(n, k)| = (-1)^{n-k} \Delta(n, k)$$

$$\left| \begin{matrix} n \\ k \end{matrix} \right| = |L(n, k)| = (-1)^{n-k} L(n, k)$$

Exercises: Prove the Following

$$\bullet \quad x^n = \sum_{k=0}^n (-1)^{n-k} \left\{ \begin{matrix} n \\ k \end{matrix} \right\} x^{(n)}$$

$$\bullet \quad (x)_n = \sum_{k=0}^n (-1)^{n-k} \left[\begin{matrix} n \\ k \end{matrix} \right] x^k$$

$$\bullet \quad (x)_n = \sum_{k=0}^n (-1)^{n-k} \left| \begin{matrix} n \\ k \end{matrix} \right| x^{(n)}$$

Theorem 1.2 :

$$\bullet \quad \sum_{j=k}^n \Delta(n, j) S(j, k) = \delta_{n,k}$$

$$\bullet \quad \sum_{j=k}^n S(n, j) \Delta(j, k) = \delta_{n,k}$$

Let $(a_n)_{n \in \mathbb{N}}$ and $(b_n)_{n \in \mathbb{N}}$ be two given sequences , then we have the following equivalence :

$$a_n = \sum_{k=0}^n (-1)^{n-k} \left[\begin{matrix} n \\ k \end{matrix} \right] b_k \iff b_n = \sum_{k=0}^n \left\{ \begin{matrix} n \\ k \end{matrix} \right\} a_k \quad (1.6)$$